---
aliases:
  - Newton's binomial theorem
tags:
  - review
  - Discrete
"References:": 
cssclasses:
  - page-theorem
sr-due: 2024-05-18
sr-interval: 1
sr-ease: 230
---
Newton’s binomial theorem describes the the algebraic expansion of power of a binomial (x-)

**Base case:**
$$(x+y)^n=\sum_{k=0}^n\binom{n}{k} x^k y^{n-k}, \quad n \geq 0 $$
**Remarks:**
$$
(1+x)^n=\sum_{k=0}^n\binom{n}{k} x^k, \quad n \geq 0 
$$
+ For every n ≥ 0
$$
\begin{aligned}
\sum_{k=0}^n\binom{n}{k} & =2^n, \\
\sum_{k=0}^n(-1)^k\binom{n}{k} & =0 .
\end{aligned}
$$
