---
aliases:
  - Logic_Submission 7
tags:
  - review
"References:": 
cssclasses:
---
3.  Transform each formula of the following deduction into a PRENEX normal form:

**first formula:**
$$
\begin{gather}
\forall x \exists y (P(x,y)\lor \lnot Q(x,y)\rightarrow R(x,y))\\\\
\forall x \exists y (\lnot[P(x,y)\lor \lnot Q(x,y)]\lor R(x,y))\\\\
\forall x \exists y ([\lnot P(x,y)\land  Q(x,y)]\lor R(x,y))\\\\
\end{gather}

$$
**second formula:**
$$
\exists x\forall y(\exists yQ(x,y)\rightarrow R(x,y))
$$
**third formula:**
$$
\exists x \exists y R(x,y)
$$
5. Transform each formula of the following deduction into a PRENEX normal form:

**first formula:**
$$
\forall x \exists y(\lnot Es(x)\land Eu(x) \rightarrow \lnot S(y,x))
$$
**second formula:**
$$
\forall x ((\forall y S(y,x) \land \lnot \exists yEs(y))\rightarrow \lnot Eu(x))
$$
8. Obtain the Skolem normal form of the equivalent formula: 
$$
\forall x \exists y \exists z [(\lnot P(x,y)\land Q(x,z))\lor R(x,y,w)]
$$
first obtain the **equivalent PRENEX normal form:**
+ No conditionals or compounded negations.  
$$

$$
9. Obtain the skolem normal form equivalent to the following formula: 
$$
\forall x [\lnot P(x,a)\rightarrow \exists yP(y,g(x))\land \forall z (P(z,g(x)) \rightarrow P(y,z)))]
$$
10. Obtain the skolem normal form equivalent to the following formula:
$$
\forall x [(P(x)\rightarrow \lnot \forall y (Q(x,y)\rightarrow \exists zP(z))) \land \forall t(Q(x,y)\rightarrow R(t))]
$$
